refactor ghost state

theories/simplang/primitive_laws.v
@@ -4,24 +4,17 @@ the Simuliris lifting lemmas. *)
 From iris.proofmode Require Export tactics.
 From iris.bi.lib Require Import fractional.
 From iris.base_logic.lib Require Import ghost_map.
-From simuliris.base_logic Require Export gen_sim_heap gen_sim_prog.
+From simuliris.base_logic Require Export gen_sim_prog.
 From simuliris.simulation Require Export slsls.
 From simuliris.simulation Require Import lifting.
-From simuliris.simplang Require Export class_instances tactics notation.
+From simuliris.simplang Require Export class_instances tactics notation ghost_state.
 From iris.prelude Require Import options.
 
-(** Allocation state for each block: either deallocated or allocated with total size n*)
-Inductive alloc_state :=
-  | DeallocSt
-  | AllocSt (n : nat).
-
 Class sheapG (Σ: gFunctors) := SHeapG {
-  sheapG_gen_heapG :> gen_sim_heapG loc loc (option (lock_state * val)) (option (lock_state * val)) Σ;
+  sheapG_gen_heapG :> heapG Σ;
   sheapG_gen_progG :> gen_sim_progG string ectx ectx Σ;
-  (* allocation size control *)
-  sheapG_ghost_mapG :> ghost_mapG Σ block alloc_state;
-  sheapG_allocN_source : gname;
-  sheapG_allocN_target : gname;
+  sheapG_allocN_source : heap_names;
+  sheapG_allocN_target : heap_names;
 }.
 
 (** This class is instantiated per proof (usually at the beginning of the file).
@@ -32,97 +25,51 @@ Class sheapInv (Σ : gFunctors) := SHeapRel {
   sheap_inv : iProp Σ;
 }.
 
-(** Allocation size control, serving as a tracker of the size of blocks and a deallocation permission for whole blocks *)
-Section alloc_size_def.
-  Context `{ghost_mapG Σ block alloc_state}.
-
-  Definition heap_alloc_rel (M : gmap block alloc_state) (σ : gmap loc (option (lock_state * val))) :=
-      (* allocations have a positive size *)
-      (∀ b l, M !! b = Some (AllocSt l) → l > 0) ∧
-      (* l is the full length of the allocation *)
-      (∀ b l, M !! b = Some (AllocSt l) → (∀ i, (∃ v, σ !! (Loc b i) = Some (Some v)) ↔ (0 ≤ i < Z.of_nat l)%Z)) ∧
-      (* deallocated*)
-      (∀ b, M !! b = Some DeallocSt → (∀ i, σ !! (Loc b i) = None ∨ σ !! (Loc b i) = Some (None))
-        (* but we need to make sure that at least one location, at offset 0, was allocated at some point before,
-           to make the bijection on heap locations work (having [Some None] allows us to use stuckness) *)
-        ∧ σ !! (Loc b 0) = Some None).
-  Definition alloc_size_interp (γ : gname) (σ : gmap loc (option (lock_state * val))) : iProp Σ :=
-    ∃ M, ghost_map_auth γ 1 M ∗ ⌜heap_alloc_rel M σ⌝.
-End alloc_size_def.
-
 Global Program Instance sheapG_simulirisG `{!sheapG Σ} `{!sheapInv Σ} : simulirisG (iPropI Σ) simp_lang := {
   state_interp P_t σ_t P_s σ_s T_s :=
     (gen_prog_interp (hG := gen_prog_inG_target) P_t ∗
      gen_prog_interp (hG := gen_prog_inG_source) P_s ∗
-     gen_heap_interp (hG := gen_heap_inG_target) σ_t.(heap) ∗
-     gen_heap_interp (hG := gen_heap_inG_source) σ_s.(heap) ∗
-     alloc_size_interp sheapG_allocN_target σ_t.(heap) ∗
-     alloc_size_interp sheapG_allocN_source σ_s.(heap) ∗
+     heap_ctx sheapG_allocN_target σ_t.(heap) σ_t.(used_blocks) ∗
+     heap_ctx sheapG_allocN_source σ_s.(heap) σ_s.(used_blocks) ∗
      sheap_inv
     )%I;
 }.
 Next Obligation. done. Qed.
 
-(** Since we use an [option val] instance of [gen_heap], we need to overwrite
-the notations.  That also helps for scopes and coercions. *)
-(** FIXME: Refactor these notations using custom entries once Coq bug #13654
-has been fixed. *)
-Notation "l '↦t{' dq } v" := (mapsto (hG:=gen_heap_inG_target) (L:=loc) (V:=option (lock_state * val)) l dq (Some (RSt 0, v%V)))
-  (at level 20, format "l  ↦t{ dq }  v") : bi_scope.
-Notation "l '↦t□' v" := (mapsto (hG:=gen_heap_inG_target) (L:=loc) (V:=option (lock_state * val)) l DfracDiscarded (Some (RSt 0, v%V)))
-  (at level 20, format "l  ↦t□  v") : bi_scope.
-Notation "l '↦t{#' q } v" := (mapsto (hG:=gen_heap_inG_target) (L:=loc) (V:=option (lock_state * val)) l (DfracOwn q) (Some (RSt 0, v%V)))
+(* TODO: add dfrac notions back if the heap supports them*)
+Notation "l '↦t[' st ']{#' q } v" := (heap_mapsto sheapG_allocN_target l st q v%V)
+  (at level 20, format "l  ↦t[ st ]{# q }  v") : bi_scope.
+Notation "l '↦t[' st ] v" := (heap_mapsto sheapG_allocN_target l st 1 v%V)
+  (at level 20, format "l  ↦t[ st ]  v") : bi_scope.
+Notation "l '↦t{#' q } v" := (heap_mapsto sheapG_allocN_target l (RSt 0) q v%V)
   (at level 20, format "l  ↦t{# q }  v") : bi_scope.
-Notation "l '↦t' v" := (mapsto (hG:=gen_heap_inG_target) (L:=loc) (V:=option (lock_state * val)) l (DfracOwn 1) (Some (RSt 0, v%V)))
+Notation "l '↦t' v" := (heap_mapsto sheapG_allocN_target l (RSt 0) 1 v%V)
   (at level 20, format "l  ↦t  v") : bi_scope.
-Notation "l '↦{' st '}t' v" := (mapsto (hG:=gen_heap_inG_target) (L:=loc) (V:=option (lock_state * val)) l (DfracOwn 1) (Some (st, v%V)))
-  (at level 20, format "l  ↦{ st }t  v") : bi_scope.
-
-Notation "l '↦s{' dq } v" := (mapsto (hG:=gen_heap_inG_source) (L:=loc) (V:=option (lock_state * val)) l dq (Some (RSt 0, v%V)))
-  (at level 20, format "l  ↦s{ dq }  v") : bi_scope.
-Notation "l '↦s□' v" := (mapsto (hG:=gen_heap_inG_source) (L:=loc) (V:=option (lock_state * val)) l DfracDiscarded (Some (RSt 0, v%V)))
-  (at level 20, format "l  ↦s□  v") : bi_scope.
-Notation "l '↦s{#' q } v" := (mapsto (hG:=gen_heap_inG_source) (L:=loc) (V:=option (lock_state * val)) l (DfracOwn q) (Some (RSt 0, v%V)))
+Notation "l '↦s[' st ']{#' q } v" := (heap_mapsto sheapG_allocN_source l st q v%V)
+  (at level 20, format "l  ↦s[ st ]{# q }  v") : bi_scope.
+Notation "l '↦s[' st ] v" := (heap_mapsto sheapG_allocN_source l st 1 v%V)
+  (at level 20, format "l  ↦s[ st ]  v") : bi_scope.
+Notation "l '↦s{#' q } v" := (heap_mapsto sheapG_allocN_source l (RSt 0) q v%V)
   (at level 20, format "l  ↦s{# q }  v") : bi_scope.
-Notation "l '↦s' v" := (mapsto (hG:=gen_heap_inG_source) (L:=loc) (V:=option (lock_state * val)) l (DfracOwn 1) (Some (RSt 0, v%V)))
+Notation "l '↦s' v" := (heap_mapsto sheapG_allocN_source l (RSt 0) 1 v%V)
   (at level 20, format "l  ↦s  v") : bi_scope.
-Notation "l '↦{' st '}s' v" := (mapsto (hG:=gen_heap_inG_source) (L:=loc) (V:=option (lock_state * val)) l (DfracOwn 1) (Some (st, v%V)))
-  (at level 20, format "l  ↦{ st }s  v") : bi_scope.
 
-(** The [array] connective is a version of [mapsto] that works with lists of values. *)
-(** [array_st] is parameterized over the individual lock states *)
-(* again parameterized over the ghost names *)
-Definition array_st `{!sheapG Σ} {γh γm} {hG : gen_heapPreNameG loc (option (lock_state * val)) Σ γh γm} (l : loc) (dq : dfrac) (vs : list val) (sts : list lock_state) : iProp Σ :=
-  ([∗ list] i ↦ v; st ∈ vs; sts, mapsto (hG:=hG) (l +ₗ i) dq (Some (st, v%V)))%I.
-Definition array `{!sheapG Σ} {γh γm} {hG : gen_heapPreNameG loc (option (lock_state * val)) Σ γh γm} (l : loc) (dq : dfrac) (vs : list val) : iProp Σ := array_st l dq vs (replicate (length vs) (RSt 0)).
-
-Lemma array_st_length_inv `{!sheapG Σ} {γh γm} {hG : gen_heapPreNameG loc (option (lock_state * val)) Σ γh γm} (l : loc) (dq : dfrac) (vs : list val) (sts : list lock_state) :
-  array_st l dq vs sts -∗ ⌜ length vs = length sts⌝.
-Proof. iApply big_sepL2_length. Qed.
-
-(** FIXME: Refactor these notations using custom entries once Coq bug #13654
-has been fixed. *)
-Notation "l ↦t∗{ dq } vs" := (array (hG:=gen_heap_inG_target) l dq vs)
-  (at level 20, format "l  ↦t∗{ dq }  vs") : bi_scope.
-Notation "l ↦t∗□ vs" := (array (hG:=gen_heap_inG_target) l DfracDiscarded vs)
-  (at level 20, format "l  ↦t∗□  vs") : bi_scope.
-Notation "l ↦t∗{# q } vs" := (array (hG:=gen_heap_inG_target) l (DfracOwn q) vs)
+Notation "l ↦t∗[ st ]{# q } vs" := (heap_mapsto_vec_st sheapG_allocN_target l st q vs)
+  (at level 20, format "l  ↦t∗[ st ]{# q }  vs") : bi_scope.
+Notation "l ↦t∗[ st ] vs" := (heap_mapsto_vec_st sheapG_allocN_target l st 1 vs)
+  (at level 20, format "l  ↦t∗[ st ]  vs") : bi_scope.
+Notation "l ↦t∗{# q } vs" := (heap_mapsto_vec sheapG_allocN_target l q vs)
   (at level 20, format "l  ↦t∗{# q }  vs") : bi_scope.
-Notation "l ↦t∗ vs" := (array (hG:=gen_heap_inG_target) l (DfracOwn 1) vs)
+Notation "l ↦t∗ vs" := (heap_mapsto_vec sheapG_allocN_target l 1 vs)
   (at level 20, format "l  ↦t∗  vs") : bi_scope.
-Notation "l '↦{' sts '}t∗' vs" := (array_st (hG:=gen_heap_inG_target) l (DfracOwn 1) vs sts)
-  (at level 20, format "l  '↦{' sts '}t∗'  vs") : bi_scope.
-
-Notation "l ↦s∗{ dq } vs" := (array (hG:=gen_heap_inG_source) l dq vs)
-  (at level 20, format "l  ↦s∗{ dq }  vs") : bi_scope.
-Notation "l ↦s∗□ vs" := (array (hG:=gen_heap_inG_source) l DfracDiscarded vs)
-  (at level 20, format "l  ↦s∗□  vs") : bi_scope.
-Notation "l ↦s∗{# q } vs" := (array (hG:=gen_heap_inG_source) l (DfracOwn q) vs)
+Notation "l ↦s∗[ st ]{# q } vs" := (heap_mapsto_vec_st sheapG_allocN_source l st q vs)
+  (at level 20, format "l  ↦s∗[ st ]{# q }  vs") : bi_scope.
+Notation "l ↦s∗[ st ] vs" := (heap_mapsto_vec_st sheapG_allocN_source l st 1 vs)
+  (at level 20, format "l  ↦s∗[ st ]  vs") : bi_scope.
+Notation "l ↦s∗{# q } vs" := (heap_mapsto_vec sheapG_allocN_source l q vs)
   (at level 20, format "l  ↦s∗{# q }  vs") : bi_scope.
-Notation "l ↦s∗ vs" := (array (hG:=gen_heap_inG_source) l (DfracOwn 1) vs)
+Notation "l ↦s∗ vs" := (heap_mapsto_vec sheapG_allocN_source l 1 vs)
   (at level 20, format "l  ↦s∗  vs") : bi_scope.
-Notation "l '↦{' sts '}s∗' vs" := (array_st (hG:=gen_heap_inG_source) l (DfracOwn 1) vs sts)
-  (at level 20, format "l  '↦{' sts '}s∗'  vs") : bi_scope.
 
 (** Program assertions *)
 Notation "f '@t' Kt" := (hasfun (hG:=gen_prog_inG_target) f Kt)
@@ -131,153 +78,18 @@ Notation "f '@s' Ks" := (hasfun (hG:=gen_prog_inG_source) f Ks)
   (at level 20, format "f  @s  Ks") : bi_scope.
 
 (** Allocation size notation *)
-Notation "l '==>s' n" := (ghost_map_elem sheapG_allocN_source (loc_chunk l) (DfracOwn 1) (AllocSt n))
-  (at level 20, format "l  ==>s  n") : bi_scope.
-Notation "l '==>t' n" := (ghost_map_elem sheapG_allocN_target (loc_chunk l) (DfracOwn 1) (AllocSt n))
-  (at level 20, format "l  ==>t  n") : bi_scope.
-Notation "'†s' l" := (ghost_map_elem sheapG_allocN_source (loc_chunk l) (DfracOwn 1) DeallocSt)
-  (at level 20, format "†s  l") : bi_scope.
-Notation "'†t' l" := (ghost_map_elem sheapG_allocN_target (loc_chunk l) (DfracOwn 1) DeallocSt)
-  (at level 20, format "†t  l") : bi_scope.
-
-Section alloc_size_laws.
-  Context `{ghost_mapG Σ block alloc_state}.
-  Lemma alloc_size_update γ (l : loc) v v' (σ : gmap loc (option (lock_state * val))) :
-    σ !! l = Some (Some v) →
-    alloc_size_interp γ σ -∗
-    alloc_size_interp γ (<[ l := Some v' ]> σ).
-  Proof.
-    iIntros (Hlookup) "Hinterp". iDestruct "Hinterp" as (M) "[Hauth %Hrel]".
-    iExists M. iFrame. iPureIntro.
-    destruct Hrel as (Hgt & Hequiv & Hdealloc). split; first done. split.
-    - intros b l' Hml i. specialize (Hequiv _ _ Hml). rewrite -Hequiv.
-      split; intros (w & Hl).
-      + destruct (decide (l = Loc b i)) as [-> | Hneq].
-        * eauto.
-        * apply lookup_insert_Some in Hl as [(Heq' & [= ->]) |[_ ?] ]; [congruence | eauto].
-      + destruct (decide (l = Loc b i)) as [-> | Hneq].
-        * exists v'. apply lookup_insert_Some; by left.
-        * exists w. apply lookup_insert_Some; by right.
-    - intros b Hml; split.
-      + intros i; specialize (proj1 (Hdealloc _ Hml) i) as [Hdealloc' | Hdealloc'].
-        * left. destruct (decide (l = Loc b i)) as [-> | Hneq]; first congruence.
-          apply lookup_insert_None; eauto.
-        * right. destruct (decide (l = Loc b i)) as [-> | Hneq]; first congruence.
-          apply lookup_insert_Some; by right.
-      + specialize (proj2 (Hdealloc _ Hml) ) as Hdealloc'.
-        destruct (decide (l = Loc b 0)) as [-> | Hneq]; first congruence.
-        apply lookup_insert_Some; by right.
-  Qed.
-
-  Lemma alloc_size_lookup_alloc γ b σ n :
-    ghost_map_elem γ b (DfracOwn 1) (AllocSt n) -∗
-    alloc_size_interp γ σ -∗
-    ⌜(∀ i, (∃ v, σ !! (Loc b i) = Some (Some v)) ↔ (0 ≤ i < Z.of_nat n)%Z) ∧ n > 0⌝.
-  Proof.
-    iIntros "Helem Hauth". iDestruct "Hauth" as (M) "[Hauth %Hrel]".
-    iDestruct (ghost_map_lookup with "Hauth Helem") as "%He". iPureIntro. split; by eapply Hrel.
-  Qed.
-
-  Lemma alloc_size_lookup_dealloc γ b σ :
-    ghost_map_elem γ b (DfracOwn 1) DeallocSt -∗
-    alloc_size_interp γ σ -∗
-    ⌜∀ i, σ !! (Loc b i) = None ∨ σ !! (Loc b i) = Some None⌝.
-  Proof.
-    iIntros "Helem Hauth". iDestruct "Hauth" as (M) "[Hauth %Hrel]".
-    iDestruct (ghost_map_lookup with "Hauth Helem") as "%He". iPureIntro. by eapply Hrel.
-  Qed.
-
-  Lemma alloc_size_free γ b σ (n : nat) :
-    ghost_map_elem γ b (DfracOwn 1) (AllocSt n) -∗
-    alloc_size_interp γ σ ==∗
-    alloc_size_interp γ (free_mem (Loc b 0) n σ) ∗ ghost_map_elem γ b (DfracOwn 1) DeallocSt.
-  Proof.
-    iIntros "Helem Hauth". iDestruct (alloc_size_lookup_alloc with "Helem Hauth") as "%Hl_prev".
-    iDestruct "Hauth" as (M) "[Hauth %Hrel]".
-    iMod (ghost_map_update DeallocSt with "Hauth Helem") as "[Hauth Helem]". iFrame.
-    iModIntro. iExists (<[b := DeallocSt]> M). iFrame "Hauth". iPureIntro.
-    destruct Hrel as (Hsize &Hrel &Hdealloc). split; [ | split].
-    - intros b' l Hl. apply lookup_insert_Some in Hl as [[_ [=]] | [_ Hl]]. by eapply Hsize.
-    - intros b' l Hl i. apply lookup_insert_Some in Hl as [[_ [=]] | [Hneq Hl]]. split.
-      + intros (w & Hlookup). apply (Hrel _ _ Hl). exists w.
-        erewrite <-lookup_free_mem_1; [done| intros [=];congruence].
-      + intros (w & Hlookup)%(Hrel _ _ Hl). exists w.
-        rewrite lookup_free_mem_1; [done | intros [=]; congruence].
-    - intros b' Hl. destruct (decide (b = b')) as [<- | Hneq].
-      + split.
-        * assert (∀ i, ¬ (0 ≤ i < n)%Z → σ !! (Loc b i) = None ∨ σ !! (Loc b i) = Some None) as Hi.
-          { intros i Hni. destruct (σ !! _) as [[] | ] eqn:Hi; [ | by eauto..].
-            contradict Hni. apply Hl_prev. eauto. }
-          intros i.
-          destruct (decide (i < 0)%Z). { rewrite lookup_free_mem_3; [ | done | cbn; lia]. apply Hi; lia. }
-          destruct (decide (i < n)%Z); first last. { rewrite lookup_free_mem_4; [ | done | cbn; lia]. apply Hi; lia. }
-          right. apply lookup_free_mem_2; [done | cbn; lia ].
-        * apply lookup_free_mem_2; [done | cbn; lia].
-      + rewrite lookup_free_mem_1; last done. split.
-        { intros i. rewrite lookup_free_mem_1; last done. apply Hdealloc.
-          apply lookup_insert_Some in Hl as [[] | [_ ?]]; done.
-        }
-        apply Hdealloc. apply lookup_insert_Some in Hl as [[] | [_ ?]]; done.
-  Qed.
-
-  Lemma heap_alloc_rel_allocN M b σ ls :
-    length ls > 0 →
-    (∀ i, σ !! (Loc b i) = None) →
-    heap_alloc_rel M σ →
-    heap_alloc_rel (<[b := AllocSt (length ls)]> M) (heap_array (Loc b 0) ls ∪ σ).
-  Proof.
-    intros Hl Hd (Hsize & Hm &Hdealloc).
-    assert (heap_array (Loc b 0) ls ##ₘ σ) as Hdisj.
-    { apply heap_array_map_disjoint. intros i Hi Hi'. apply Hd. }
-    split.
-    { intros b' n [[<- [= <-]] | [_ Hs]]%lookup_insert_Some; first done. by eapply Hsize. }
-    split.
-    { intros b' n. rewrite lookup_insert_Some.
-      intros [[<- [= <-]] | [? Hs]] i.
-      - split.
-        + intros (v & [Hlookup | Hlookup]%lookup_union_Some); last done.
-          * apply heap_array_lookup in Hlookup as (j & w & ? & Heq & [= ->] & ?).
-            inversion Heq; subst. apply list_lookup_alt in H3 as (? & _). lia.
-          * exfalso. congruence.
-        + intros [H1 H2]. exists (RSt 0, (ls !!! (Z.to_nat i))).
-          apply lookup_union_Some_l. apply heap_array_lookup.
-          exists i, (ls !!! Z.to_nat i). repeat split; [done | ].
-          apply list_lookup_lookup_total_lt. lia.
-      - split.
-        + intros (v & [Hlookup | Hlookup]%lookup_union_Some); last done.
-          * exfalso. apply heap_array_lookup in Hlookup as (j & w & ? & ? & [= ->] & ?).
-            inversion H3; subst. congruence.
-          * apply (Hm _ _ Hs); eauto.
-        + intros (v & Hi)%(Hm _ _ Hs). exists v. apply lookup_union_Some_r; done.
-    }
-    { intros b'. rewrite lookup_insert_Some. intros [[_ [=]] | [Hneq Hlookup]]; split.
-      - intros i; rewrite lookup_union_r; first by eapply Hdealloc.
-        destruct (heap_array _ _ !! _) eqn:Heq; last done.
-        apply heap_array_lookup in Heq as (j & w & ? & [=] & ?); congruence.
-      - rewrite lookup_union_r; first by eapply Hdealloc.
-        destruct (heap_array _ _ !! _) eqn:Heq; last done.
-        apply heap_array_lookup in Heq as (j & w & ? & [=] & ?); congruence.
-    }
-  Qed.
-
-  Lemma alloc_size_allocN γ b σ ls :
-    length ls > 0 →
-    (∀ i, σ !! (Loc b i) = None) →
-    alloc_size_interp γ σ ==∗
-    alloc_size_interp γ (heap_array (Loc b 0) ls ∪ σ) ∗
-    ghost_map_elem γ b (DfracOwn 1) (AllocSt (length ls)).
-  Proof.
-    iIntros (Hl Hd) "Hi". iDestruct "Hi" as (M) "(Hauth & %Hsize & %Hm & %Hdealloc)".
-    iMod (ghost_map_insert b (AllocSt (length ls)) with "Hauth") as "[Hauth $]".
-    { destruct (M !! b) eqn:Hlookup; last done. destruct a.
-      - specialize (Hdealloc _ Hlookup) as [_ Hdealloc]. congruence.
-      - specialize (Hm _ _ Hlookup) as Hm1. specialize (Hsize _ _ Hlookup).
-        destruct (proj2 (Hm1 0) ltac:(lia)). specialize (Hd 0). congruence.
-    }
-    iModIntro. iExists (<[b := AllocSt (length ls)]> M). iFrame "Hauth". iPureIntro.
-    by apply heap_alloc_rel_allocN.
-  Qed.
-End alloc_size_laws.
+Notation "† l '…?t' n" := (heap_freeable sheapG_allocN_target l 1 n)
+  (at level 20, format "† l …?t  n") : bi_scope.
+Notation "† l '…t' n" := (heap_freeable sheapG_allocN_target l 1 (Some n))
+  (at level 20, format "† l …t  n") : bi_scope.
+Notation "† l '…t' -" := (heap_freeable sheapG_allocN_target l 1 None)
+  (at level 20, format "† l …t  -") : bi_scope.
+Notation "† l '…?s' n" := (heap_freeable sheapG_allocN_source l 1 n)
+  (at level 20, format "† l …?s  n") : bi_scope.
+Notation "† l '…s' n" := (heap_freeable sheapG_allocN_source l 1 (Some n))
+  (at level 20, format "† l …s  n") : bi_scope.
+Notation "† l '…s' -" := (heap_freeable sheapG_allocN_source l 1 None)
+  (at level 20, format "† l …s  -") : bi_scope.
 
 
 Section lifting.
@@ -293,259 +105,6 @@ Implicit Types π : thread_id.
 Context (Ω : val → val → iProp Σ) (π : thread_id).
 Local Notation "et '⪯' es [{ Φ }]" := (et ⪯{π, Ω} es [{Φ}])%I (at level 40, Φ at level 200) : bi_scope.
 
-
-(** Heap for target *)
-
-(** We need to adjust the [gen_heap] lemmas because of our
-value type being [option val]. *)
-
-Lemma mapsto_target_valid l dq v : l ↦t{dq} v -∗ ⌜✓ dq⌝.
-Proof. apply mapsto_valid. Qed.
-Lemma mapsto_target_valid_2 l dq1 dq2 v1 v2 :
-  l ↦t{dq1} v1 -∗ l ↦t{dq2} v2 -∗ ⌜✓ (dq1 ⋅ dq2) ∧ v1 = v2⌝.
-Proof.
-  iIntros "H1 H2". iDestruct (mapsto_valid_2 with "H1 H2") as %[? [=?]]. done.
-Qed.
-Lemma mapsto_target_agree l dq1 dq2 v1 v2 : l ↦t{dq1} v1 -∗ l ↦t{dq2} v2 -∗ ⌜v1 = v2⌝.
-Proof. iIntros "H1 H2". iDestruct (mapsto_agree with "H1 H2") as %[=?]. done. Qed.
-
-Lemma mapsto_target_combine l dq1 dq2 v1 v2 :
-  l ↦t{dq1} v1 -∗ l ↦t{dq2} v2 -∗ l ↦t{dq1 ⋅ dq2} v1 ∗ ⌜v1 = v2⌝.
-Proof.
-  iIntros "Hl1 Hl2". iDestruct (mapsto_combine with "Hl1 Hl2") as "[$ Heq]".
-  by iDestruct "Heq" as %[= ->].
-Qed.
-
-Lemma mapsto_target_frac_ne l1 l2 dq1 dq2 v1 v2 :
-  ¬ ✓(dq1 ⋅ dq2) → l1 ↦t{dq1} v1 -∗ l2 ↦t{dq2} v2 -∗ ⌜l1 ≠ l2⌝.
-Proof. apply mapsto_frac_ne. Qed.
-Lemma mapsto_target_ne l1 l2 dq2 v1 v2 : l1 ↦t v1 -∗ l2 ↦t{dq2} v2 -∗ ⌜l1 ≠ l2⌝.
-Proof. apply mapsto_ne. Qed.
-
-Lemma mapsto_target_persist l dq v : l ↦t{dq} v ==∗ l ↦t□ v.
-Proof. apply mapsto_persist. Qed.
-
-(** Heap for source *)
-
-Lemma mapsto_source_valid l dq v : l ↦s{dq} v -∗ ⌜✓ dq⌝.
-Proof. apply mapsto_valid. Qed.
-Lemma mapsto_source_valid_2 l dq1 dq2 v1 v2 :
-  l ↦s{dq1} v1 -∗ l ↦s{dq2} v2 -∗ ⌜✓ (dq1 ⋅ dq2) ∧ v1 = v2⌝.
-Proof.
-  iIntros "H1 H2". iDestruct (mapsto_valid_2 with "H1 H2") as %[? [=?]]. done.
-Qed.
-Lemma mapsto_source_agree l dq1 dq2 v1 v2 : l ↦s{dq1} v1 -∗ l ↦s{dq2} v2 -∗ ⌜v1 = v2⌝.
-Proof. iIntros "H1 H2". iDestruct (mapsto_agree with "H1 H2") as %[=?]. done. Qed.
-
-Lemma mapsto_source_combine l dq1 dq2 v1 v2 :
-  l ↦s{dq1} v1 -∗ l ↦s{dq2} v2 -∗ l ↦s{dq1 ⋅ dq2} v1 ∗ ⌜v1 = v2⌝.
-Proof.
-  iIntros "Hl1 Hl2". iDestruct (mapsto_combine with "Hl1 Hl2") as "[$ Heq]".
-  by iDestruct "Heq" as %[= ->].
-Qed.
-
-Lemma mapsto_source_frac_ne l1 l2 dq1 dq2 v1 v2 :
-  ¬ ✓(dq1 ⋅ dq2) → l1 ↦s{dq1} v1 -∗ l2 ↦s{dq2} v2 -∗ ⌜l1 ≠ l2⌝.
-Proof. apply mapsto_frac_ne. Qed.
-Lemma mapsto_source_ne l1 l2 dq2 v1 v2 : l1 ↦s v1 -∗ l2 ↦s{dq2} v2 -∗ ⌜l1 ≠ l2⌝.
-Proof. apply mapsto_ne. Qed.
-
-Lemma mapsto_source_persist l dq v : l ↦s{dq} v ==∗ l ↦s□ v.
-Proof. apply mapsto_persist. Qed.
-
-(** Array lemmas *)
-Lemma target_array_st_access vs sts (i : nat) v st l :
-  vs !! i = Some v →
-  sts !! i = Some st →
-  l ↦{sts}t∗ vs -∗
-  (l +ₗ i) ↦{st}t v ∗ (∀ v' st', (l +ₗ i) ↦{st'}t v' -∗ l ↦{<[i := st']> sts}t∗ <[i := v']>vs).
-Proof.
-  iIntros (Hsome_v Hsome_st) "Hs".
-  rewrite /array_st. iApply (big_sepL2_insert_acc _ _ _ i v st Hsome_v Hsome_st with "Hs").
-Qed.
-
-Lemma source_array_st_access vs sts (i : nat) v st l :
-  vs !! i = Some v →
-  sts !! i = Some st →
-  l ↦{sts}s∗ vs -∗
-  (l +ₗ i) ↦{st}s v ∗ (∀ v' st', (l +ₗ i) ↦{st'}s v' -∗ l ↦{<[i := st']> sts}s∗ <[i := v']>vs).
-Proof.
-  iIntros (Hsome_v Hsome_st) "Hs".
-  rewrite /array_st. iApply (big_sepL2_insert_acc _ _ _ i v st Hsome_v Hsome_st with "Hs").
-Qed.
-
-Lemma target_array_access vs (i : nat) v l :
-  vs !! i = Some v →
-  l ↦t∗ vs -∗
-  (l +ₗ i) ↦t v ∗ (∀ v', (l +ₗ i) ↦t v' -∗ l ↦t∗ <[i := v']>vs).
-Proof.
-  iIntros (Hsome) "Hs". rewrite /array.
-  iPoseProof (target_array_st_access vs (replicate (length vs) (RSt 0)) i v (RSt 0) l with "Hs") as "[$ Ha]"; first done.
-  { apply lookup_replicate; split; [done | ]. by eapply list_lookup_alt. }
-  iIntros (v') "Hv'". iSpecialize ("Ha" $! v' (RSt 0) with "Hv'").
-  by rewrite insert_replicate insert_length.
-Qed.
-
-Lemma source_array_access vs (i : nat) v l :
-  vs !! i = Some v →
-  l ↦s∗ vs -∗
-  (l +ₗ i) ↦s v ∗ (∀ v', (l +ₗ i) ↦s v' -∗ l ↦s∗ <[i := v']>vs).
-Proof.
-  iIntros (Hsome) "Hs". rewrite /array.
-  iPoseProof (source_array_st_access vs (replicate (length vs) (RSt 0)) i v (RSt 0) l with "Hs") as "[$ Ha]"; first done.
-  { apply lookup_replicate; split; [done | ]. by eapply list_lookup_alt. }
-  iIntros (v') "Hv'". iSpecialize ("Ha" $! v' (RSt 0) with "Hv'").
-  by rewrite insert_replicate insert_length.
-Qed.
-
-Lemma source_array_st_access' vs sts l :
-  (0 ≤ loc_idx l < length vs)%Z →
-  (Loc (loc_chunk l) 0) ↦{sts}s∗ vs -∗
-  l ↦{sts !!! Z.to_nat (loc_idx l)}s (vs !!! Z.to_nat (loc_idx l)) ∗
-  (∀ v' st', l ↦{st'}s v' -∗ (Loc (loc_chunk l) 0) ↦{<[Z.to_nat (loc_idx l) := st']> sts}s∗ (<[Z.to_nat (loc_idx l) := v']> vs)).
-Proof.
-  iIntros (Hsome) "Hs".
-  iPoseProof (array_st_length_inv with "Hs") as "%Hl".
-  iPoseProof (source_array_st_access _ _ (Z.to_nat (loc_idx l)) with "Hs") as "[Hl_s Hclose_s]".
-  { apply list_lookup_alt. split; last reflexivity. lia. }
-  { apply list_lookup_alt. split; last reflexivity. lia. }
-  rewrite Loc_add. assert (Z.of_nat (Z.to_nat (loc_idx l))= loc_idx l) as -> by lia. rewrite loc_eta.
-  iFrame.
-Qed.
-
-Lemma target_array_st_access' vs sts l :
-  (0 ≤ loc_idx l < length vs)%Z →
-  (Loc (loc_chunk l) 0) ↦{sts}t∗ vs -∗
-  l ↦{sts !!! Z.to_nat (loc_idx l)}t (vs !!! Z.to_nat (loc_idx l)) ∗
-  (∀ v' st', l ↦{st'}t v' -∗ (Loc (loc_chunk l) 0) ↦{<[Z.to_nat (loc_idx l) := st']> sts}t∗ (<[Z.to_nat (loc_idx l) := v']> vs)).
-Proof.
-  iIntros (Hsome) "Hs".
-  iPoseProof (array_st_length_inv with "Hs") as "%Hl".
-  iPoseProof (target_array_st_access _ _ (Z.to_nat (loc_idx l)) with "Hs") as "[Hl_s Hclose_s]".
-  { apply list_lookup_alt. split; last reflexivity. lia. }
-  { apply list_lookup_alt. split; last reflexivity. lia. }
-  rewrite Loc_add. assert (Z.of_nat (Z.to_nat (loc_idx l))= loc_idx l) as -> by lia. rewrite loc_eta.
-  iFrame.
-Qed.
-
-Lemma source_array_access' vs l :
-  (0 ≤ loc_idx l < length vs)%Z →
-  (Loc (loc_chunk l) 0) ↦s∗ vs -∗
-  l ↦s (vs !!! Z.to_nat (loc_idx l)) ∗ (∀ v', l ↦s v' -∗ (Loc (loc_chunk l) 0) ↦s∗ (<[Z.to_nat (loc_idx l) := v']> vs)).
-Proof.
-  iIntros (Hsome) "Hs".
-  iPoseProof (source_array_access _ (Z.to_nat (loc_idx l)) with "Hs") as "[Hl_s Hclose_s]".
-  { apply list_lookup_alt. split; last reflexivity. lia. }
-  rewrite Loc_add. assert (Z.of_nat (Z.to_nat (loc_idx l))= loc_idx l) as -> by lia. rewrite loc_eta.
-  iFrame.
-Qed.
-
-Lemma target_array_access' vs l :
-  (0 ≤ loc_idx l < length vs)%Z →
-  (Loc (loc_chunk l) 0) ↦t∗ vs -∗
-  l ↦t (vs !!! Z.to_nat (loc_idx l)) ∗ (∀ v', l ↦t v' -∗ (Loc (loc_chunk l) 0) ↦t∗ (<[Z.to_nat (loc_idx l) := v']> vs)).
-Proof.
-  iIntros (Hsome) "Hs".
-  iPoseProof (target_array_access _ (Z.to_nat (loc_idx l)) with "Hs") as "[Hl_s Hclose_s]".
-  { apply list_lookup_alt. split; last reflexivity. lia. }
-  rewrite Loc_add. assert (Z.of_nat (Z.to_nat (loc_idx l))= loc_idx l) as -> by lia. rewrite loc_eta.
-  iFrame.
-Qed.
-
-(** Alloc for source *)
-Lemma alloc_source_ne l1 l2 n1 n2 : l1 ==>s n1 -∗ l2 ==>s n2 -∗ ⌜loc_chunk l1 ≠ loc_chunk l2⌝.
-Proof. iIntros "Hn1 Hn2". iApply (ghost_map_elem_ne with "Hn1 Hn2"). Qed.
-
-Lemma alloc_source_offset l n i : l ==>s n -∗ (l +ₗ i) ==>s n.
-Proof. done. Qed.
-
-Lemma alloc_source_lt l n σ : alloc_size_interp sheapG_allocN_source (σ.(heap)) -∗ l ==>s n -∗ ⌜0 < n⌝.
-Proof.
-  iIntros "Hinterp Hn".
-  iDestruct "Hinterp" as (M) "(Hauth  & %Hs & _)".
-  iPoseProof (ghost_map_lookup with "Hauth Hn") as "%Ha".
-  iPureIntro. by eapply Hs.
-Qed.
-
-Lemma alloc_source_dealloc l n : l ==>s n -∗ †s l -∗ False.
-Proof. iIntros "Hn1 Hn2". iPoseProof (ghost_map_elem_agree with "Hn1 Hn2") as "%Ha". iPureIntro; congruence. Qed.
-
-(* We can learn that l's index must be 0, if it points to the full allocation. *)
-Lemma alloc_source_seq_start n vs l σ :
-  n = length vs →
-  alloc_size_interp sheapG_allocN_source (σ.(heap)) -∗
-  gen_heap_interp (hG := gen_heap_inG_source) σ.(heap) -∗
-  l ==>s n -∗
-  l ↦s∗ vs -∗
-  ⌜loc_idx l = 0⌝.
-Proof.
-  iIntros (->) "Ha Hσ Halloc Hl".
-  iPoseProof (alloc_size_lookup_alloc with "Halloc Ha") as "%Hs".
-  iAssert (∀ i, ⌜(0 ≤ i < length vs)%Z⌝ → ⌜∃ w, heap σ !! (l +ₗ i) = Some (Some w)⌝)%I with "[Hσ Hl]" as "Hhea".
-  { iIntros (i) "%Hrange".
-    iPoseProof (source_array_access _ (Z.to_nat i) with "Hl") as "[Hs _]".
-    { apply list_lookup_alt; split; [lia | reflexivity]. }
-    iDestruct (gen_heap_valid with "Hσ Hs") as %?. iPureIntro.
-    replace (Z.of_nat (Z.to_nat i)) with i in H by lia. eauto.
-  }
-  destruct Hs as [Hs ?].
-  destruct (decide (loc_idx l < 0)%Z) as [Hlt | Hnlt].
-  { iPoseProof ("Hhea" $! 0 with "[]") as "%Heh"; first by iPureIntro; lia.
-    exfalso. destruct l; cbn in*. apply Hs in Heh. cbn in Heh. lia.
-  }
-  destruct (decide (loc_idx l > 0)%Z) as [Hgt | Hngt]; last by iPureIntro; lia.
-  iPoseProof ("Hhea" $! (pred (length vs)) with "[]") as "%Heh"; first by iPureIntro; lia.
-  exfalso. destruct l; cbn in*. apply Hs in Heh. cbn in Heh. lia.
-Qed.
-
-
-(** Alloc for target *)
-Lemma alloc_target_ne l1 l2 n1 n2 : l1 ==>t n1 -∗ l2 ==>t n2 -∗ ⌜loc_chunk l1 ≠ loc_chunk l2⌝.
-Proof. iIntros "Hn1 Hn2". iApply (ghost_map_elem_ne with "Hn1 Hn2"). Qed.
-
-Lemma alloc_target_offset l n i : l ==>t n -∗ (l +ₗ i) ==>t n.
-Proof. done. Qed.
-
-Lemma alloc_target_lt l n σ : alloc_size_interp sheapG_allocN_target (σ.(heap)) -∗ l ==>t n -∗ ⌜0 < n⌝.
-Proof.
-  iIntros "Hinterp Hn".
-  iDestruct "Hinterp" as (M) "(Hauth  & %Hs & _)".
-  iPoseProof (ghost_map_lookup with "Hauth Hn") as "%Ha".
-  iPureIntro. by eapply Hs.
-Qed.
-
-Lemma alloc_target_dealloc l n : l ==>t n -∗ †t l -∗ False.
-Proof. iIntros "Hn1 Hn2". iPoseProof (ghost_map_elem_agree with "Hn1 Hn2") as "%Ha". iPureIntro; congruence. Qed.
-
-Lemma alloc_target_seq_start n vs l σ :
-  n = length vs →
-  alloc_size_interp sheapG_allocN_target σ.(heap) -∗
-  gen_heap_interp (hG := gen_heap_inG_target) σ.(heap) -∗
-  l ==>t n -∗
-  l ↦t∗ vs -∗
-  ⌜loc_idx l = 0⌝.
-Proof.
-  iIntros (->) "Ha Hσ Halloc Hl".
-  iPoseProof (alloc_size_lookup_alloc with "Halloc Ha") as "%Hs".
-  iAssert (∀ i, ⌜(0 ≤ i < length vs)%Z⌝ → ⌜∃ w, heap σ !! (l +ₗ i) = Some (Some w)⌝)%I with "[Hσ Hl]" as "Hhea".
-  { iIntros (i) "%Hrange".
-    iPoseProof (target_array_access _ (Z.to_nat i) with "Hl") as "[Hs _]".
-    { apply list_lookup_alt; split; [lia | reflexivity]. }
-    iDestruct (gen_heap_valid with "Hσ Hs") as %?. iPureIntro.
-    replace (Z.of_nat (Z.to_nat i)) with i in H by lia. eauto.
-  }
-  destruct Hs as [Hs ?].
-  destruct (decide (loc_idx l < 0)%Z) as [Hlt | Hnlt].
-  { iPoseProof ("Hhea" $! 0 with "[]") as "%Heh"; first by iPureIntro; lia.
-    exfalso. destruct l; cbn in*. apply Hs in Heh. cbn in Heh. lia.
-  }
-  destruct (decide (loc_idx l > 0)%Z) as [Hgt | Hngt]; last by iPureIntro; lia.
-  iPoseProof ("Hhea" $! (pred (length vs)) with "[]") as "%Heh"; first by iPureIntro; lia.
-  exfalso. destruct l; cbn in*. apply Hs in Heh. cbn in Heh. lia.
-Qed.
-
-
-
 (** Program for target *)
 Lemma hasfun_target_agree f K_t1 K_t2 : f @t K_t1 -∗ f @t K_t2 -∗ ⌜K_t1 = K_t2⌝.
 Proof. apply hasfun_agree. Qed.
@@ -556,300 +115,180 @@ Proof. apply hasfun_agree. Qed.
 
 
 (** operational heap lemmas *)
-Lemma heap_array_to_seq_mapsto l v (n : nat) γh γm (hG : gen_heapPreNameG loc (option (lock_state * val)) Σ γh γm) :
-  ([∗ map] l' ↦ ov ∈ heap_array l (replicate n v), gen_sim_heap.mapsto (hG:=hG) l' (DfracOwn 1) ov) -∗
-  [∗ list] i ∈ seq 0 n, gen_sim_heap.mapsto (hG:=hG) (l +ₗ (i : nat)) (DfracOwn 1) (Some (RSt 0, v)).
-Proof.
-  iIntros "Hvs". iInduction n as [|n] "IH" forall (l); simpl.
-  { done. }
-  rewrite big_opM_union; last first.
-  { apply map_disjoint_spec=> l' v1 v2 /lookup_singleton_Some [-> _].
-    intros (j&w&?&Hjl&_)%heap_array_lookup.
-    rewrite loc_add_assoc -{1}[l']loc_add_0 in Hjl. simplify_eq; lia. }
-  rewrite loc_add_0 -fmap_S_seq big_sepL_fmap.
-  setoid_rewrite Nat2Z.inj_succ. setoid_rewrite <-Z.add_1_l.
-  setoid_rewrite <-loc_add_assoc.
-  rewrite big_opM_singleton; iDestruct "Hvs" as "[$ Hvs]". by iApply "IH".
-Qed.
 
-Lemma target_red_allocN_seq n v Ψ :
+Lemma target_red_allocN n v Ψ :
   (0 < n)%Z →
-  (∀ l, ([∗ list] i ∈ seq 0 (Z.to_nat n), (l +ₗ (i : nat)) ↦t v) -∗
-    l ==>t (Z.to_nat n) -∗ target_red (of_val #l) Ψ) -∗
+  (∀ l, l ↦t∗ (replicate (Z.to_nat n) v) -∗
+    † l …t (Z.to_nat n) -∗ target_red (of_val #l) Ψ) -∗
   target_red (AllocN (Val $ LitV $ LitInt $ n) (Val v)) Ψ.
 Proof.
   iIntros (Hn) "Hloc". iApply target_red_lift_head_step.
-  iIntros (P_s σ_s P_t σ_t T_s) "(HP_t & HP_s & Hσ_t & Hσ_s & Ha_t & Ha_s & Hinv)". iModIntro.
+  iIntros (P_s σ_s P_t σ_t T_s) "(HP_t & HP_s & Hσ_t & Hσ_s & Hinv)". iModIntro.
   iSplitR. { eauto using alloc_fresh with head_step. }
   iIntros (e_t' efs_t σ_t') "%"; inv_head_step.
   set (l := Loc b 0).
-  iMod (gen_heap_alloc_big _ (heap_array l (replicate (Z.to_nat n) v)) with "Hσ_t")
-    as "(Hσ_t & Hl & _)".
-  { apply heap_array_map_disjoint. rewrite replicate_length Z2Nat.id; rewrite /loc_add; auto with lia.  }
-  iPoseProof (heap_array_to_seq_mapsto with "Hl") as "Hmap".
-  iFrame.
-  iMod (alloc_size_allocN _ b (σ_t.(heap)) (replicate (Z.to_nat n) v) with "Ha_t") as "(Ha_t & Hn)";
-    [rewrite replicate_length; lia | done | ].
+  iMod (heap_alloc _ _ l with "Hσ_t") as "($&Hn&Hm)"; [done..|].
   iModIntro. iFrame. iSplitR; first done.
-  rewrite replicate_length. iApply ("Hloc" with "Hmap Hn").
+  by iApply ("Hloc" with "Hm Hn").
 Qed.
 
-Lemma source_red_allocN_seq n v Ψ:
+Lemma source_red_allocN n v Ψ:
   (0 < n)%Z →
-  (∀ l, ([∗ list] i ∈ seq 0 (Z.to_nat n), (l +ₗ (i : nat)) ↦s v) -∗
-  l ==>s (Z.to_nat n) -∗ source_red (of_val #l) π Ψ) -∗
+  (∀ l, l ↦s∗ (replicate (Z.to_nat n) v) -∗
+  † l …s Z.to_nat n -∗ source_red (of_val #l) π Ψ) -∗
   source_red (AllocN (Val $ LitV $ LitInt $ n) (Val v)) π Ψ.
 Proof.
   iIntros (Hn) "Hloc". iApply source_red_lift_head_step.
-  iIntros (P_s σ_s P_t σ_t T_s K_s) "[(HP_t & HP_s & Hσ_t & Hσ_s & Ha_t & Ha_s & Hinv) _]".
-  assert (head_reducible P_s (AllocN #n v) σ_s) as (e_s' & σ_s' & efs & Hred).
-  { eauto using alloc_fresh with lia head_step. }
-  inv_head_step. (set l := Loc b 0).
-  iMod (gen_heap_alloc_big _ (heap_array l (replicate (Z.to_nat n) v)) with "Hσ_s")
-    as "(Hσ_s & Hl & Hm)".
-  { apply heap_array_map_disjoint. rewrite replicate_length Z2Nat.id /loc_add; auto with lia. }
-  iModIntro. iExists #l, (state_init_heap l n v σ_s).
-  iSplitR. { eauto with lia head_step. }
-  iFrame.
-  iMod (alloc_size_allocN _ b (σ_s.(heap)) (replicate (Z.to_nat n) v) with "Ha_s") as "(Ha_s & Hn)";
-    [rewrite replicate_length; lia | done | ].
-  iModIntro. iFrame. rewrite replicate_length.
-  iApply ("Hloc" with "[Hl] [Hn]"); last done. iApply (heap_array_to_seq_mapsto with "Hl").
+  iIntros (P_s σ_s P_t σ_t T_s K_s) "[(HP_t & HP_s & Hσ_t & Hσ_s & Hinv) _]".
+  iExists _, _. iSplitR. { simpl. eauto using alloc_fresh with lia head_step. }
+  simpl.
+  iMod (heap_alloc _ _ (Loc (fresh_block (heap σ_s) (used_blocks σ_s)) 0) with "Hσ_s") as "($&Hn&Hm)"; [done|done| | |].
+  { apply is_fresh_block_blocks. }
+  { move => ?. apply is_fresh_block. }
+  iModIntro. iFrame.
+  by iApply ("Hloc" with "Hm Hn").
 Qed.
 
 Lemma target_red_alloc v Ψ :
-  (∀ l, l ↦t v -∗ l ==>t 1 -∗ target_red (of_val #l) Ψ) -∗
+  (∀ l, l ↦t v -∗ † l …t 1 -∗ target_red (of_val #l) Ψ) -∗
   target_red (Alloc (Val v)) Ψ.
 Proof.
-  iIntros "Ht". iApply (target_red_allocN_seq); first lia.
-  iIntros (l) "[Hl _]". iApply "Ht". by rewrite loc_add_0.
+  iIntros "Ht". iApply (target_red_allocN); first lia.
+  have ->: (Z.to_nat 1 = 1) by lia. simpl.
+  iIntros (l). rewrite heap_mapsto_vec_singleton. iApply "Ht".
 Qed.
 
 Lemma source_red_alloc v Ψ :
-  (∀ l, l ↦s v -∗ l ==>s 1 -∗ source_red (of_val #l) π Ψ) -∗
+  (∀ l, l ↦s v -∗ † l …s 1 -∗ source_red (of_val #l) π Ψ) -∗
   source_red (Alloc (Val v)) π Ψ.
 Proof.
-  iIntros "Ht". iApply (source_red_allocN_seq); first lia.
-  iIntros (l) "[Hl _]". iApply "Ht". by rewrite loc_add_0.
+  iIntros "Ht". iApply (source_red_allocN); first lia.
+  have ->: (Z.to_nat 1 = 1) by lia. simpl.
+  iIntros (l). rewrite heap_mapsto_vec_singleton. iApply "Ht".
 Qed.
 
-Lemma heap_array_st_validN {γh γm} {hG : gen_heapPreNameG loc (option (lock_state * val)) Σ γh γm} σ vs sts n l :
-  length vs = Z.to_nat n →
-  gen_heap_interp (hG := hG) σ.(heap) -∗
-  array_st (hG := hG) l (DfracOwn 1) vs sts -∗
-  ⌜∀ i, (0 ≤ i < n)%Z → σ.(heap) !! (l +ₗ i) = Some (Some (sts !!! (Z.to_nat i), vs !!! (Z.to_nat i)))⌝.
-Proof.
-  iIntros (Hn) "Hσ Hl".
-  iPoseProof (array_st_length_inv with "Hl") as "%Hlen".
-  iInduction vs as [] "IH" forall (n l sts Hlen Hn); cbn in Hn.
-  - iPureIntro. intros i ?. lia.
-  - destruct sts as [ | b sts]; [cbn in Hlen; lia |].
-    rewrite /array_st big_sepL2_cons loc_add_0. iDestruct "Hl" as "[Hl0 Hlr]".
-    iDestruct (gen_heap_valid with "Hσ Hl0") as "%Hs".
-    iPoseProof ("IH" $! (Z.pred n) (l +ₗ 1) sts with "[] [] Hσ [Hlr]") as "%IH".
-    + iPureIntro; cbn in Hlen. lia.
-    + iPureIntro. lia.
-    + iApply (big_sepL2_mono with "Hlr").
-      intros k v st Hv Hst; simpl. rewrite loc_add_assoc. replace (Z.of_nat (S k)) with (1 + k)%Z; [done | lia].
-    + iPureIntro. intros i Hi. destruct (decide (i = 0)) as [-> | ].
-      { rewrite loc_add_0. eauto. }
-      specialize (IH (Z.pred i) ltac:(lia)) as IH.
-      rewrite !lookup_total_cons_ne_0; [ | lia | lia].
-      replace (Nat.pred (Z.to_nat i)) with (Z.to_nat (Z.pred i)) by lia.
-      rewrite -IH. rewrite loc_add_assoc. by replace (1 + Z.pred i)%Z with i%Z by lia.
-Qed.
-
-Lemma heap_array_validN {γh γm} {hG : gen_heapPreNameG loc (option (lock_state * val)) Σ γh γm} σ vs n l :
-  length vs = Z.to_nat n →
-  gen_heap_interp (hG := hG) σ.(heap) -∗
-  array (hG := hG) l (DfracOwn 1) vs -∗
-  ⌜∀ i, (0 ≤ i < n)%Z → σ.(heap) !! (l +ₗ i) = Some (Some (RSt 0, vs !!! (Z.to_nat i)))⌝.
-Proof.
-  iIntros (Hn) "Hσ Hl".
-  iPoseProof (heap_array_st_validN with "Hσ Hl") as "%Ha"; first done.
-  iPureIntro. intros i Hi. rewrite (Ha i Hi).
-  rewrite lookup_total_replicate_2; [done | lia].
-Qed.
-
-Lemma heap_array_st_freeN {γh γm} {hG : gen_heapPreNameG loc (option (lock_state * val)) Σ γh γm} σ vs sts n l :
-  length vs = n →
-  gen_heap_interp (hG:=hG) σ.(heap) -∗
-  array_st (hG := hG) l (DfracOwn 1) vs sts ==∗
-  gen_heap_interp (hG:=hG) (free_mem l n σ.(heap)).
-Proof.
-  iIntros (<-) "Hσ Hl". iPoseProof (array_st_length_inv with "Hl") as "%Hl".
-  iInduction vs as [] "IH" forall (l σ sts Hl); first done.
-  destruct sts as [ | st sts]; [ cbn in Hl; lia | ].
-  rewrite /array_st big_sepL2_cons loc_add_0. iDestruct "Hl" as "[Hl0 Hlr]".
-  iMod (gen_heap_update _ _ _ None with "Hσ Hl0") as "[Hσ _]".
-  iMod ("IH" $! (l +ₗ 1) (state_upd_heap <[l:=None]> σ) sts with "[] Hσ [Hlr]") as "IH'".
-  - iPureIntro; cbn in Hl; lia.
-  - iApply (big_sepL2_mono with "Hlr").
-    intros k v st' Ha Hst'; simpl. rewrite loc_add_assoc. replace (Z.of_nat (S k)) with (1 + k)%Z; [done | lia].
-  - iModIntro. cbn. rewrite (upd_free_mem σ l _ 1); last lia. iApply "IH'".
-Qed.
-
-Lemma target_red_freeN vs l n Ψ :
-  length vs = (Z.to_nat n) →
+Lemma target_red_freeN vs l (n : Z) Ψ :
+  n = length vs →
   l ↦t∗ vs -∗
-  l ==>t (Z.to_nat n) -∗
-  target_red (of_val #()) Ψ -∗
+  † l …t Z.to_nat n -∗
+  († l …t - -∗ target_red (of_val #()) Ψ) -∗
   target_red (FreeN (Val $ LitV $ LitInt n) (Val $ LitV (LitLoc l))) Ψ.
 Proof.
-  iIntros (Hn) "Hl Hn Hsim". iApply target_red_lift_head_step.
-  iIntros (?????) "(HP_t & HP_s & Hσ_t & Hσ_s & Ha_t & Ha_s & Hinv)".
-  iPoseProof (alloc_size_lookup_alloc with "Hn Ha_t") as "%Halloc".
-  iPoseProof (alloc_target_lt with "Ha_t Hn") as "%Hlt".
-  iPoseProof (alloc_target_seq_start with "Ha_t Hσ_t Hn Hl") as "%Hidx_lt"; first done.
-  iPoseProof (heap_array_validN with "Hσ_t Hl") as "%Hv"; first done.
-  iModIntro.
-  assert (∀ i, (0 ≤ i < n)%Z → ∃ v, heap σ_t !! (l +ₗ i) = Some (Some (RSt 0, v))) as Hi1 by eauto.
-  assert (∀ i, (∃ v st, heap σ_t !! (l +ₗ i) = Some (Some (st, v))) → (0 ≤ i < n)%Z) as Hi2.
-  { intros i (v &st & Hv0). replace (Z.of_nat (Z.to_nat n)) with n in Halloc by lia. apply Halloc.
-      exists (st, v). destruct l; rewrite /loc_add Hidx_lt in Hv0; cbn in *.
-      replace (0%nat + i)%Z with i in Hv0 by lia. apply Hv0.
-  }
+  iIntros (->) "Hl Hn Hsim". iApply target_red_lift_head_step. rewrite Nat2Z.id.
+  iIntros (?????) "(HP_t & HP_s & Hσ_t & Hσ_s & Hinv)".
+  rewrite heap_mapsto_vec_to_st.
+  iMod (heap_free with "Hσ_t Hl Hn") as (??) "[? ?]"; [ done| ].
   iSplitR; first by eauto with lia head_step.
-  iIntros (e_t' efs σ_t') "%"; inv_head_step.
-
-  iMod (alloc_size_free with "Hn Ha_t") as "[Ha_t Hn]". iFrame.
-  iMod (heap_array_st_freeN with "Hσ_t Hl") as "$"; first done.
-  iModIntro. iSplitR; first done.
-  assert (Loc (loc_chunk l) 0 = l) as ->.
-  { destruct l; cbn in *; rewrite Hidx_lt. replace 0%Z with (Z.of_nat 0); done. }
-  done.
+  iIntros "!>" (e_t' efs σ_t') "%"; inv_head_step.
+  iModIntro. iFrame. iSplitR; first done. by iApply "Hsim".
 Qed.
 
 Lemma target_red_free v l Ψ :
   l ↦t v -∗
-  l ==>t 1 -∗
-  target_red (of_val #()) Ψ -∗
+  † l …t 1 -∗
+  († l …t - -∗ target_red (of_val #()) Ψ) -∗
   target_red (FreeN (Val $ LitV $ LitInt 1) (Val $ LitV (LitLoc l))) Ψ.
 Proof.
   iIntros "Hl Hn". replace (1) with (Z.to_nat 1) by lia.
-  iApply (target_red_freeN [v] with "[Hl] Hn"); first done.
-  cbn. rewrite loc_add_0; eauto.
+  iApply (target_red_freeN [v] with "[Hl] [Hn]"); [ done..| |done].
+  by rewrite heap_mapsto_vec_singleton.
 Qed.
 
-Lemma source_red_freeN vs l n Ψ :
-  length vs = (Z.to_nat n) →
+Lemma source_red_freeN vs l (n : Z) Ψ :
+  n = length vs →
   l ↦s∗ vs -∗
-  l ==>s (Z.to_nat n) -∗
-  source_red (of_val #()) π Ψ -∗
+  † l …s (Z.to_nat n) -∗
+  († l …s - -∗ source_red (of_val #()) π Ψ) -∗
   source_red (FreeN (Val $ LitV $ LitInt n) (Val $ LitV (LitLoc l))) π Ψ.
 Proof.
-  iIntros (Hn) "Hl Hn Hsim". iApply source_red_lift_head_step.
-  iIntros (??????) "[(HP_t & HP_s & Hσ_t & Hσ_s & Ha_t & Ha_s & Hinv) _]".
-  iPoseProof (alloc_size_lookup_alloc with "Hn Ha_s") as "%Halloc".
-  iPoseProof (alloc_source_lt with "Ha_s Hn") as "%Hlt".
-  iPoseProof (alloc_source_seq_start with "Ha_s Hσ_s Hn Hl") as "%Hidx_lt"; first done.
-  iPoseProof (heap_array_validN with "Hσ_s Hl") as "%Hv"; first done.
-  iModIntro.
-  assert (∀ i, (0 ≤ i < n)%Z → ∃ v, heap σ_s !! (l +ₗ i) = Some (Some (RSt 0, v))) as Hi1 by eauto.
-  assert (∀ i, (∃ v st, heap σ_s !! (l +ₗ i) = Some (Some (st, v))) → (0 ≤ i < n)%Z) as Hi2.
-  { intros i (v &st & Hv0). replace (Z.of_nat (Z.to_nat n)) with n in Halloc by lia. apply Halloc.
-      exists (st, v). destruct l; rewrite /loc_add Hidx_lt in Hv0; cbn in *.
-      replace (0%nat + i)%Z with i in Hv0 by lia. apply Hv0.
-  }
-  iExists (Val #()), (state_upd_heap (free_mem l (Z.to_nat n)) σ_s).
+  iIntros (->) "Hl Hn Hsim". iApply source_red_lift_head_step. rewrite Nat2Z.id.
+  iIntros (??????) "[(HP_t & HP_s & Hσ_t & Hσ_s & Hinv) _]".
+  rewrite heap_mapsto_vec_to_st.
+  iMod (heap_free with "Hσ_s Hl Hn") as (??) "[? ?]"; [ done | ].
+  iExists (Val #()), (state_upd_heap (free_mem l _) σ_s).
   iSplitR; first eauto with lia head_step.
   { iPureIntro. econstructor; eauto with lia. }
-
-  iMod (alloc_size_free with "Hn Ha_s") as "[Ha_s Hn]". iFrame.
-  iMod (heap_array_st_freeN with "Hσ_s Hl") as "$"; first done.
-  iModIntro.
-  assert (Loc (loc_chunk l) 0 = l) as ->.
-  { destruct l; cbn in *; rewrite Hidx_lt. replace 0%Z with (Z.of_nat 0); done. }
-  done.
+  iModIntro. iModIntro. iFrame. by iApply "Hsim".
 Qed.
 
 Lemma source_red_free v l Ψ :
   l ↦s v -∗
-  l ==>s 1 -∗
-  source_red (of_val #()) π Ψ -∗
+  † l …s 1 -∗
+  († l …s - -∗ source_red (of_val #()) π Ψ) -∗
   source_red (FreeN (Val $ LitV $ LitInt 1) (Val $ LitV (LitLoc l))) π Ψ.
 Proof.
   iIntros "Hl Hn". replace (1) with (Z.to_nat 1) by lia.
-  iApply (source_red_freeN [v] with "[Hl] Hn"); first done.
-  cbn. rewrite loc_add_0; eauto.
+  iApply (source_red_freeN [v] with "[Hl] Hn"); [ done.. |].
+  by rewrite heap_mapsto_vec_singleton.
 Qed.
 
-Lemma target_red_load_sc l dq v Ψ :
-  l ↦t{dq} v -∗
-  (l ↦t{dq} v -∗ target_red (of_val v) Ψ) -∗
+Lemma target_red_load_sc l q v Ψ :
+  l ↦t{#q} v -∗
+  (l ↦t{#q} v -∗ target_red (of_val v) Ψ) -∗
   target_red (Load ScOrd (Val $ LitV $ LitLoc l)) Ψ.
 Proof.
   iIntros "Hl Ht". iApply target_red_lift_head_step.
   iIntros (?????) "(HP_t & HP_s & Hσ_t & Hσ_s & Hinv)".
-  iDestruct (gen_heap_valid with "Hσ_t Hl") as %?. iModIntro.
+  iDestruct (heap_read with "Hσ_t Hl") as %[??]. iModIntro.
   iSplit; first by eauto with head_step.
   iIntros (??? Hstep); inv_head_step.
   iModIntro. iFrame. iSplit;[done|]. by iApply "Ht".
 Qed.
 
-(** FIXME: this is not the theorem we would like as the lock_state does currently not interact well with fractions *)
-Lemma target_red_load_na l v Ψ :
-  l ↦t v -∗
-  (l ↦t v -∗ target_red (of_val v) Ψ) -∗
+Lemma target_red_load_na l q v Ψ :
+  l ↦t{#q} v -∗
+  (l ↦t{#q} v -∗ target_red (of_val v) Ψ) -∗
   target_red (Load Na1Ord (Val $ LitV $ LitLoc l)) Ψ.
 Proof.
   iIntros "Hl Ht". iApply target_red_lift_head_step.
-  iIntros (?????) "(HP_t & HP_s & Hσ_t & Hσ_s & Ha_t & Ha_s & Hinv)".
-  iDestruct (gen_heap_valid with "Hσ_t Hl") as %?. iModIntro.
+  iIntros (?????) "(HP_t & HP_s & Hσ_t & Hσ_s & Hinv)".
+  iMod (heap_read_na with "Hσ_t Hl") as (n ?) "[Hσ_t Hcont]". iModIntro.
   iSplit; first by eauto with head_step.
-  iIntros (??? Hstep); inv_head_step.
-  iMod (gen_heap_update with "Hσ_t Hl") as "[$ Hl]".
-  iDestruct (alloc_size_update with "Ha_t") as "$"; first done.
-  iModIntro. iFrame. iSplitR; first done.
+  iIntros (??? Hstep) "!>"; inv_head_step.
+  iFrame. iSplitR; [done|].
 
   iApply target_red_lift_head_step.
-  iIntros (?????) "(HP_t & HP_s & Hσ_t & Hσ_s & Ha_t & Ha_s & Hinv)".
-  iDestruct (gen_heap_valid with "Hσ_t Hl") as %?. iModIntro.
+  iIntros (?????) "(HP_t & HP_s & Hσ_t & Hσ_s & Hinv)".
+  iMod ("Hcont" with "Hσ_t") as (? ?) "[Hσ_t Hm]". iModIntro.
   iSplit; first by eauto with head_step.
-  iIntros (??? Hstep); inv_head_step.
-  iMod (gen_heap_update with "Hσ_t Hl") as "[$ Hl]".
-  iDestruct (alloc_size_update with "Ha_t") as "$"; first done.
-  iModIntro. iFrame. iSplitR; first done. by iApply "Ht".
+  iIntros (??? Hstep) "!>"; inv_head_step.
+  iFrame. iSplitR; [done|].
+  by iApply "Ht".
 Qed.
 
-Lemma source_red_load_sc l dq v Ψ :
-  l ↦s{dq} v -∗
-  (l ↦s{dq} v -∗ source_red (of_val v) π Ψ) -∗
+Lemma source_red_load_sc l q v Ψ :
+  l ↦s{#q} v -∗
+  (l ↦s{#q} v -∗ source_red (of_val v) π Ψ) -∗
   source_red (Load ScOrd (Val $ LitV $ LitLoc l)) π Ψ.
 Proof.
   iIntros "Hl Ht". iApply source_red_lift_head_step.
   iIntros (??????) "[(HP_t & HP_s & Hσ_t & Hσ_s & Hinv) _]".
-  iDestruct (gen_heap_valid with "Hσ_s Hl") as %?.
+  iDestruct (heap_read with "Hσ_s Hl") as %[??]. iModIntro.
   assert (∃ e_s' σ_s', head_step P_s (Load ScOrd #l) σ_s e_s' σ_s' []) as (e_s' & σ_s' & Hred).
   { eauto with head_step. }
-  iModIntro; iExists e_s', σ_s'. iSplit; first by eauto. inv_head_step.
+  iExists e_s', σ_s'. iSplit; first by eauto. inv_head_step.
   iModIntro. iFrame. by iApply "Ht".
 Qed.
 
-(** FIXME: this is not the theorem we would like as the lock_state does currently not interact well with fractions *)
-Lemma source_red_load_na l v Ψ :
-  l ↦s v -∗
-  (l ↦s v -∗ source_red (of_val v) π Ψ) -∗
+Lemma source_red_load_na l v Ψ q :
+  l ↦s{#q} v -∗
+  (l ↦s{#q} v -∗ source_red (of_val v) π Ψ) -∗
   source_red (Load Na1Ord (Val $ LitV $ LitLoc l)) π Ψ.
 Proof.
   iIntros "Hl Ht". iApply source_red_lift_head_step.
-  iIntros (??????) "[(HP_t & HP_s & Hσ_t & Hσ_s & Ha_t & Ha_s & Hinv) _]".
-  iDestruct (gen_heap_valid with "Hσ_s Hl") as %?.
+  iIntros (??????) "[(HP_t & HP_s & Hσ_t & Hσ_s & Hinv) _]".
+  iMod (heap_read_na with "Hσ_s Hl") as (n ?) "[Hσ_s Hcont]". iModIntro.
   assert (∃ e_s' σ_s', head_step P_s (Load Na1Ord #l) σ_s e_s' σ_s' []) as (e_s' & σ_s' & Hred).
   { eauto with head_step. }
-  iModIntro; iExists e_s', σ_s'. iSplit; first by eauto. inv_head_step.
-  iMod (gen_heap_update with "Hσ_s Hl") as "[$ Hl]".
-  iDestruct (alloc_size_update with "Ha_s") as "$"; first done.
+  iExists e_s', σ_s'. iSplit; first by eauto. inv_head_step.
   iModIntro. iFrame.
 
   iApply source_red_lift_head_step.
-  iIntros (??????) "[(HP_t & HP_s & Hσ_t & Hσ_s & Ha_t & Ha_s & Hinv) _]".
-  iDestruct (gen_heap_valid with "Hσ_s Hl") as %?.
+  iIntros (??????) "[(HP_t & HP_s & Hσ_t & Hσ_s & Hinv) _]".
+  iMod ("Hcont" with "Hσ_s") as (? ?) "[Hσ_s Hm]". iModIntro.
   assert (∃ e_s' σ_s', head_step P_s0 (Load Na2Ord #l) σ_s0 e_s' σ_s' []) as (e_s' & σ_s' & Hred).
   { eauto with lia head_step. }
-  iModIntro; iExists e_s', σ_s'. iSplit; first by eauto. inv_head_step.
-  iMod (gen_heap_update with "Hσ_s Hl") as "[$ Hl]".
-  iDestruct (alloc_size_update with "Ha_s") as "$"; first done.
+  iExists e_s', σ_s'. iSplit; first by eauto. inv_head_step.
   iModIntro. iFrame.
   by iApply "Ht".
 Qed.
@@ -860,13 +299,12 @@ Lemma target_red_store_sc l v v' Ψ :
   target_red (Store ScOrd (Val $ LitV (LitLoc l)) (Val v)) Ψ.
 Proof.
   iIntros "Hl Hsim". iApply target_red_lift_head_step.
-  iIntros (?????) "(HP_t & HP_s & Hσ_t & Hσ_s & Ha_t & Ha_s & Hinv) !>".
-  iDestruct (gen_heap_valid with "Hσ_t Hl") as %?.
+  iIntros (?????) "(HP_t & HP_s & Hσ_t & Hσ_s & Hinv) !>".
+  iDestruct (heap_read_1 with "Hσ_t Hl") as %?.
   iSplitR; first by eauto with head_step.
   iIntros (e_t' efs σ_t') "%"; inv_head_step.
-  iMod (gen_heap_update with "Hσ_t Hl") as "[$ Hl]".
-  iFrame. iDestruct (alloc_size_update with "Ha_t") as "$"; first done.
-  iModIntro. iSplitR; first done. by iApply "Hsim".
+  iMod (heap_write with "Hσ_t Hl") as "[$ ?]".
+  iFrame. iModIntro. iSplitR; first done. by iApply "Hsim".
 Qed.
 
 Lemma target_red_store_na l v v' Ψ :
@@ -875,22 +313,19 @@ Lemma target_red_store_na l v v' Ψ :
   target_red (Store Na1Ord (Val $ LitV (LitLoc l)) (Val v)) Ψ.
 Proof.
   iIntros "Hl Hsim". iApply target_red_lift_head_step.
-  iIntros (?????) "(HP_t & HP_s & Hσ_t & Hσ_s & Ha_t & Ha_s & Hinv) !>".
-  iDestruct (gen_heap_valid with "Hσ_t Hl") as %?.
-  iSplitR; first by eauto with head_step.
-  iIntros (e_t' efs σ_t') "%"; inv_head_step.
-  iMod (gen_heap_update with "Hσ_t Hl") as "[$ Hl]".
-  iFrame. iDestruct (alloc_size_update with "Ha_t") as "$"; first done.
-  iModIntro. iSplitR; first done.
+  iIntros (?????) "(HP_t & HP_s & Hσ_t & Hσ_s & Hinv)".
+  iMod (heap_write_na with "Hσ_t Hl") as (?) "[Hσ_t Hcont]". iModIntro.
+  iSplit; first by eauto with head_step.
+  iIntros (??? Hstep) "!>"; inv_head_step.
+  iFrame. iSplitR; [done|].
 
   iApply target_red_lift_head_step.
-  iIntros (?????) "(HP_t & HP_s & Hσ_t & Hσ_s & Ha_t & Ha_s & Hinv) !>".
-  iDestruct (gen_heap_valid with "Hσ_t Hl") as %?.
-  iSplitR; first by eauto with head_step.
-  iIntros (e_t' efs σ_t') "%"; inv_head_step.
-  iMod (gen_heap_update with "Hσ_t Hl") as "[$ Hl]".
-  iFrame. iDestruct (alloc_size_update with "Ha_t") as "$"; first done.
-  iModIntro. iSplitR; first done. by iApply "Hsim".
+  iIntros (?????) "(HP_t & HP_s & Hσ_t & Hσ_s & Hinv)".
+  iMod ("Hcont" with "Hσ_t") as (?) "[Hσ_t Hm]". iModIntro.
+  iSplit; first by eauto with head_step.
+  iIntros (??? Hstep) "!>"; inv_head_step.
+  iFrame. iSplitR; [done|].
+  by iApply "Hsim".
 Qed.
 
 Lemma source_red_store_sc l v v' Ψ :
@@ -899,14 +334,13 @@ Lemma source_red_store_sc l v v' Ψ :
   source_red (Store ScOrd (Val $ LitV (LitLoc l)) (Val v)) π Ψ.
 Proof.
   iIntros "Hl Hsim". iApply source_red_lift_head_step.
-  iIntros (??????) "[(HP_t & HP_s & Hσ_t & Hσ_s & Ha_t & Ha_s & Hinv) _] !>".
-  iDestruct (gen_heap_valid with "Hσ_s Hl") as %?.
+  iIntros (??????) "[(HP_t & HP_s & Hσ_t & Hσ_s & Hinv) _] !>".
+  iDestruct (heap_read_1 with "Hσ_s Hl") as %?.
   assert (∃ e_s' σ_s', head_step P_s (Store ScOrd (Val $ LitV (LitLoc l)) (Val v)) σ_s e_s' σ_s' []) as (e_s' & σ_s' & Hred).
   { eauto with head_step. }
   iExists e_s', σ_s'. iSplitR; first done. inv_head_step.
-  iMod (gen_heap_update with "Hσ_s Hl") as "[$ Hl]".
-  iFrame. iDestruct (alloc_size_update with "Ha_s") as "$"; first done.
-  iModIntro. by iApply "Hsim".
+  iMod (heap_write with "Hσ_s Hl") as "[$ ?]".
+  iFrame. iModIntro. by iApply "Hsim".
 Qed.
 
 Lemma source_red_store_na l v v' Ψ :
@@ -915,25 +349,21 @@ Lemma source_red_store_na l v v' Ψ :
   source_red (Store Na1Ord (Val $ LitV (LitLoc l)) (Val v)) π Ψ.
 Proof.
   iIntros "Hl Hsim". iApply source_red_lift_head_step.
-  iIntros (??????) "[(HP_t & HP_s & Hσ_t & Hσ_s & Ha_t & Ha_s & Hinv) _] !>".
-  iDestruct (gen_heap_valid with "Hσ_s Hl") as %?.
+  iIntros (??????) "[(HP_t & HP_s & Hσ_t & Hσ_s & Hinv) _]".
+  iMod (heap_write_na with "Hσ_s Hl") as (?) "[Hσ_s Hcont]". iModIntro.
   assert (∃ e_s' σ_s', head_step P_s (Store Na1Ord (Val $ LitV (LitLoc l)) (Val v)) σ_s e_s' σ_s' [])
     as (e_s' & σ_s' & Hred).
   { eauto with head_step. }
   iExists e_s', σ_s'. iSplitR; first done. inv_head_step.
-  iMod (gen_heap_update with "Hσ_s Hl") as "[$ Hl]".
-  iFrame. iDestruct (alloc_size_update with "Ha_s") as "$"; first done.
-  iModIntro.
+  iModIntro. iFrame.
 
   iApply source_red_lift_head_step.
-  iIntros (??????) "[(HP_t & HP_s & Hσ_t & Hσ_s & Ha_t & Ha_s & Hinv) _] !>".
-  iDestruct (gen_heap_valid with "Hσ_s Hl") as %?.
+  iIntros (??????) "[(HP_t & HP_s & Hσ_t & Hσ_s & Hinv) _]".
+  iMod ("Hcont" with "Hσ_s") as (?) "[Hσ_s Hm]". iModIntro.
   assert (∃ e_s' σ_s', head_step P_s0 (Store Na2Ord (Val $ LitV (LitLoc l)) (Val v)) σ_s0 e_s' σ_s' []) as (e_s' & σ_s' & Hred).
   { eauto with head_step. }
   iExists e_s', σ_s'. iSplitR; first done. inv_head_step.
-  iMod (gen_heap_update with "Hσ_s Hl") as "[$ Hl]".
-  iFrame. iDestruct (alloc_size_update with "Ha_s") as "$"; first done.
-  iModIntro. by iApply "Hsim".
+  iModIntro. iFrame. by iApply "Hsim".
 Qed.
 
 (** operational lemmas for calls *)
